code/k256/Hacl.Impl.K256.PointDouble.fst
@@ -22,6 +22,94 @@ open Hacl.Impl.K256.Point
 
 
 inline_for_extraction noextract
+val calc_z3 (y1 z1 z3 yy tmp:felem) : Stack unit
+  (requires fun h ->
+    live h y1 /\ live h z1 /\ live h z3 /\
+    live h yy /\ live h tmp /\
+    disjoint y1 z1 /\ disjoint y1 z3 /\ disjoint y1 yy /\
+    disjoint y1 tmp /\ eq_or_disjoint z1 z3 /\ disjoint z1 yy /\
+    disjoint z1 tmp /\ disjoint z3 yy /\ disjoint z3 tmp /\ disjoint yy tmp /\
+
+    inv_lazy_reduced2 h y1 /\ inv_lazy_reduced2 h z1 /\ inv_lazy_reduced2 h yy)
+  (ensures  fun h0 _ h1 -> modifies (loc tmp |+| loc z3) h0 h1 /\
+    feval h1 z3 = S.fmul (S.fmul (S.fmul (feval h0 yy) (feval h0 y1)) (feval h0 z1)) 8 /\
+    inv_lazy_reduced2 h1 z3)
+
+let calc_z3 y1 z1 z3 yy tmp =
+  fmul tmp yy y1; //tmp = yy*y
+  fmul z3 tmp z1; //z3 = tmp*z = yy*y*z
+  let h1 = ST.get () in
+  //assert (inv_lazy_reduced2 h1 x3);
+  //assert (inv_lazy_reduced2 h1 tmp);
+  //assert (inv_lazy_reduced2 h1 z3);
+
+  fmul_8_normalize_weak z3 z3 //z3 = z3*8=yy*y*z*8
+
+
+inline_for_extraction noextract
+val calc_bzz9_tmp (yy zz bzz3 bzz9 tmp:felem) : Stack unit
+  (requires fun h ->
+    live h yy /\ live h zz /\ live h bzz3 /\ live h bzz9 /\ live h tmp /\
+    disjoint yy zz /\ disjoint yy bzz3 /\ disjoint yy bzz9 /\
+    disjoint yy tmp /\ disjoint zz bzz3 /\ disjoint zz bzz9 /\
+    disjoint zz tmp /\ disjoint bzz3 bzz9 /\ disjoint bzz3 tmp /\
+    disjoint bzz9 tmp /\
+    inv_lazy_reduced2 h yy /\ inv_lazy_reduced2 h zz)
+  (ensures  fun h0 _ h1 ->
+    modifies (loc bzz3 |+| loc bzz9 |+| loc tmp) h0 h1 /\
+    (let bzz3 = S.fmul (S.fmul 3 S.b) (feval h0 zz) in
+     feval h1 bzz9 = S.fsub (feval h0 yy) (S.fmul 3 bzz3) /\
+     feval h1 tmp = S.fmul (feval h1 bzz9) (S.fadd (feval h0 yy) bzz3) /\
+     inv_lazy_reduced2 h1 tmp /\ felem_fits5 (as_felem5 h1 bzz9) (13,13,13,13,14)))
+
+let calc_bzz9_tmp yy zz bzz3 bzz9 tmp =
+  fmul_3b_normalize_weak bzz3 zz; //bzz3 = (3*b)*zz
+  let h1 = ST.get () in
+  //assert (inv_lazy_reduced2 h1 bzz3);
+
+  fmul_small_num bzz9 bzz3 (u64 3); //bzz9 = 3*bzz3
+  let h2 = ST.get () in
+  BL.fmul15_lemma (1,1,1,1,2) 3 (as_felem5 h1 bzz3) (u64 3);
+  //assert (felem_fits5 (as_felem5 h2 bzz9) (3,3,3,3,6));
+
+  BL.fsub5_lemma (1,1,1,1,2) (3,3,3,3,6) (as_felem5 h1 yy) (as_felem5 h2 bzz9) (u64 6);
+  fsub bzz9 yy bzz9 (u64 6); //bzz9 = yy_m_bzz9 = yy-bzz9
+  let h3 = ST.get () in
+  //assert (felem_fits5 (as_felem5 h3 bzz9) (13,13,13,13,14));
+
+  fadd tmp yy bzz3; //tmp = yy_p_bzz3 = yy+bzz3
+  let h4 = ST.get () in
+  BL.fadd5_lemma (1,1,1,1,2) (1,1,1,1,2) (as_felem5 h1 yy) (as_felem5 h1 bzz3);
+  //assert (felem_fits5 (as_felem5 h4 tmp) (2,2,2,2,4));
+
+  fmul tmp bzz9 tmp //tmp = bzz9*tmp = yy_m_bzz9*yy_p_bzz3
+
+
+inline_for_extraction noextract
+val calc_y3 (y3 tmp: felem) : Stack unit
+  (requires fun h ->
+    live h y3 /\ live h tmp /\ disjoint y3 tmp /\
+    inv_lazy_reduced2 h y3 /\ inv_lazy_reduced2 h tmp)
+  (ensures  fun h0 _ h1 -> modifies (loc y3) h0 h1 /\
+    feval h1 y3 = S.fadd (feval h0 tmp) (S.fmul (S.fmul 24 S.b) (feval h0 y3))/\
+    inv_lazy_reduced2 h1 y3)
+
+let calc_y3 y3 tmp =
+  let h0 = ST.get () in
+  fmul_small_num y3 y3 (u64 168); //y3 = t = (24*b)*y3 = (24*b)*yy_zz
+  let h1 = ST.get () in
+  BL.fmul15_lemma (1,1,1,1,2) 168 (as_felem5 h0 y3) (u64 168);
+  //assert (felem_fits5 (as_felem5 h1 y3) (168,168,168,168,336));
+
+  fadd y3 tmp y3;  //y3 = tmp+y3 = yy_m_bzz9*yy_p_bzz3+t
+  let h2 = ST.get () in
+  BL.fadd5_lemma (1,1,1,1,2) (168,168,168,168,336) (as_felem5 h0 tmp) (as_felem5 h1 y3);
+  //assert (felem_fits5 (as_felem5 h2 y3) (169,169,169,169,338));
+  fnormalize_weak y3 y3;
+  BL.normalize_weak5_lemma (169,169,169,169,338) (as_felem5 h2 y3)
+
+
+inline_for_extraction noextract
 val point_double_no_alloc (out p:point) (tmp:lbuffer uint64 (5ul *! nlimb)) : Stack unit
   (requires fun h ->
     live h out /\ live h p /\ live h tmp /\
@@ -53,55 +141,12 @@ let point_double_no_alloc out p tmp =
   //assert (felem_fits5 (as_felem5 h2 x3) (2,2,2,2,4));
 
   fmul x3 x3 y1; //x3 = xy2 = x3*y = (2*x)*y
-  fmul tmp yy y1; //tmp = yy*y
-  fmul z3 tmp z1; //z3 = tmp*z = yy*y*z
-  let h3 = ST.get () in
-  //assert (inv_lazy_reduced2 h3 x3);
-  //assert (inv_lazy_reduced2 h3 tmp);
-  //assert (inv_lazy_reduced2 h3 z3);
-
-  fmul_8_normalize_weak z3 z3; //z3 = z3*8=yy*y*z*8
-  fmul_3b_normalize_weak bzz3 zz; //bzz3 = (3*b)*zz
-  let h5 = ST.get () in
-  //assert (inv_lazy_reduced2 h5 z3);
-  //assert (inv_lazy_reduced2 h5 bzz3);
-
-  fmul_small_num bzz9 bzz3 (u64 3); //bzz9 = 3*bzz3
-  let h6 = ST.get () in
-  BL.fmul15_lemma (1,1,1,1,2) 3 (as_felem5 h5 bzz3) (u64 3);
-  //assert (felem_fits5 (as_felem5 h6 bzz9) (3,3,3,3,6));
-
-  BL.fsub5_lemma (1,1,1,1,2) (3,3,3,3,6) (as_felem5 h6 yy) (as_felem5 h6 bzz9) (u64 6);
-  fsub bzz9 yy bzz9 (u64 6); //bzz9 = yy_m_bzz9 = yy-bzz9
-  let h7 = ST.get () in
-  //assert (felem_fits5 (as_felem5 h7 bzz9) (13,13,13,13,14));
-
-  fadd tmp yy bzz3; //tmp = yy_p_bzz3 = yy+bzz3
-  let h8 = ST.get () in
-  BL.fadd5_lemma (1,1,1,1,2) (1,1,1,1,2) (as_felem5 h7 yy) (as_felem5 h7 bzz3);
-  //assert (felem_fits5 (as_felem5 h8 tmp) (2,2,2,2,4));
+  calc_z3 y1 z1 z3 yy tmp;
+  calc_bzz9_tmp yy zz bzz3 bzz9 tmp;
 
   fmul y3 yy zz; //y3 = yy_zz = yy*zz
-  let h9 = ST.get () in
-  //assert (inv_lazy_reduced2 h9 y3);
-
-  fmul_small_num y3 y3 (u64 168); //y3 = t = (24*b)*y3 = (24*b)*yy_zz
-  let h10 = ST.get () in
-  BL.fmul15_lemma (1,1,1,1,2) 168 (as_felem5 h9 y3) (u64 168);
-  //assert (felem_fits5 (as_felem5 h10 y3) (168,168,168,168,336));
-
   fmul x3 x3 bzz9; //x3 = x3*bzz9 = xy2*yy_m_bzz9
-  fmul tmp bzz9 tmp; //tmp = bzz9*tmp = yy_m_bzz9*yy_p_bzz3
-  let h11 = ST.get () in
-  //assert (inv_lazy_reduced2 h11 x3);
-  //assert (inv_lazy_reduced2 h11 tmp);
-
-  fadd y3 tmp y3;  //y3 = tmp+y3 = yy_m_bzz9*yy_p_bzz3+t
-  let h12 = ST.get () in
-  BL.fadd5_lemma (1,1,1,1,2) (168,168,168,168,336) (as_felem5 h11 tmp) (as_felem5 h11 y3);
-  //assert (felem_fits5 (as_felem5 h12 y3) (169,169,169,169,338));
-  fnormalize_weak y3 y3;
-  BL.normalize_weak5_lemma (169,169,169,169,338) (as_felem5 h12 y3)
+  calc_y3 y3 tmp
 
 
 val point_double (out p:point) : Stack unit
